template-coq/theories/Universes.v
@@ -699,7 +699,7 @@ End Universe.
 Definition is_propositional u := 
   Universe.is_prop u || Universe.is_sprop u.
 
-Definition relevance_of_sort s := if (Universe.is_sprop s) then Irrelevant else Relevant.
+Definition relevance_of_sort `{checker_flags} s := if (check_univs && Universe.is_sprop s) then Irrelevant else Relevant.
 
 (** This coercion allows to see the universes as a [UnivExprSet.t] *)
 Coercion Universe.t_set : Universe.nonEmptyUnivExprSet >-> UnivExprSet.t.
@@ -2217,14 +2217,22 @@ Section no_prop_leq_type.
 End no_prop_leq_type.
 
 Lemma leq_relevance {cf φ} {s1 s2} :
-  check_univs -> consistent φ -> leq_universe φ s1 s2 -> relevance_of_sort s1 = relevance_of_sort s2.
+  consistent φ -> leq_universe φ s1 s2 -> relevance_of_sort s1 = relevance_of_sort s2.
 Proof.
-  intros Hcf c H.
+  intros c H.
+  destruct check_univs eqn:Hc.
   enough (Universe.is_sprop s1 <-> Universe.is_sprop s2).
   destruct s1, s2, H0 as [H1 H2]; cbn in H1, H2 |- *; try reflexivity;
   assert true by auto; intuition auto; discriminate.
   split; [eapply leq_universe_sprop_l | eapply leq_universe_sprop_r]; eauto.
+  unfold relevance_of_sort; rewrite Hc. reflexivity.
 Qed.
+
+Theorem relevance_subst {cf} u s : relevance_of_sort (subst_instance_univ u s) = relevance_of_sort s.
+Proof.
+  destruct s; reflexivity.
+Qed.
+
 
 Definition compare_universe {cf:checker_flags} (pb : conv_pb) :=
   match pb with
