pcuic/theories/PCUICRelevance.v
@@ -1,6 +1,2 @@
 From MetaCoq.PCUIC Require Import PCUICAst.
 
-Theorem relevance_subst u s : relevance_of_sort (subst_instance_univ u s) = relevance_of_sort s.
-Proof.
-  destruct s; reflexivity.
-Qed.
