template-coq/theories/Reduction.v
@@ -17,7 +17,7 @@ Proof.
   apply app_red_l. auto.
 Qed.
 
-Lemma red1_mkApp Σ Γ M1 N1 M2 :
+Lemma red1_mkApp `{cf: checker_flags} Σ Γ M1 N1 M2 :
   WfAst.wf Σ M1 ->
   red1 Σ Γ M1 N1 -> red1 Σ Γ (mkApp M1 M2) (mkApp N1 M2).
 Proof.
@@ -45,7 +45,7 @@ Proof.
   now apply red1_tApp_mkApp.
 Qed.
 
-Lemma red1_mkApps_l Σ Γ M1 N1 M2 :
+Lemma red1_mkApps_l `{cf: checker_flags} Σ Γ M1 N1 M2 :
   WfAst.wf Σ M1 -> All (WfAst.wf Σ) M2 ->
   red1 Σ Γ M1 N1 -> red1 Σ Γ (mkApps M1 M2) (mkApps N1 M2).
 Proof.
@@ -59,7 +59,7 @@ Proof.
   apply red1_mkApp; auto.
 Qed.
 
-Lemma red1_mkApps_r Σ Γ M1 M2 N2 :
+Lemma red1_mkApps_r `{cf: checker_flags} Σ Γ M1 M2 N2 :
   WfAst.wf Σ M1 -> All (WfAst.wf Σ) M2 ->
   OnOne2 (red1 Σ Γ) M2 N2 -> red1 Σ Γ (mkApps M1 M2) (mkApps M1 N2).
 Proof.
